src/invariant/Invariant.v
@@ -37,7 +37,7 @@ Definition ThreadsProp :=
     Prop.
 
 Definition MemoryProp :=
-  forall (assign: FLocFun.t Const.t),
+  forall (assign: LocFun.t Const.t),
     Prop.
 
 
@@ -54,7 +54,7 @@ Module Logic.
           forall tid lang syn
             (FIND: IdentMap.find tid program = Some (existT _ lang syn)),
             S tid lang (lang.(Language.init) syn)>> /\
-        <<ASSIGN_INIT: J (FLocFun.init 0)>>;
+        <<ASSIGN_INIT: J (LocFun.init 0)>>;
       SILENT:
         forall tid lang st1 st2
           (ST1: S tid lang st1)
@@ -65,7 +65,7 @@ Module Logic.
           loc val ord
           assign
           (ST1: S tid lang st1)
-          (ASSIGN1: J assign /\ FLocFun.find loc assign = val)
+          (ASSIGN1: J assign /\ LocFun.find loc assign = val)
           (STEP: lang.(Language.step) (ProgramEvent.read loc val ord) st1 st2),
           S tid lang st2;
       WRITE:
@@ -74,16 +74,16 @@ Module Logic.
           (ST1: S tid lang st1)
           (STEP: lang.(Language.step) (ProgramEvent.write loc val ord) st1 st2),
           <<ST2: S tid lang st2>> /\
-          <<ASSIGN2: forall assign, J assign -> J (FLocFun.add loc val assign)>>;
+          <<ASSIGN2: forall assign, J assign -> J (LocFun.add loc val assign)>>;
       UPDATE:
         forall tid lang st1 st2
           loc valr valw ordr ordw
           assign
           (ST1: S tid lang st1)
-          (ASSIGN1: J assign /\ FLocFun.find loc assign = valr)
+          (ASSIGN1: J assign /\ LocFun.find loc assign = valr)
           (STEP: lang.(Language.step) (ProgramEvent.update loc valr valw ordr ordw) st1 st2),
           <<ST2: S tid lang st2>> /\
-          <<ASSIGN2: forall assign, J assign -> J (FLocFun.add loc valw assign)>>;
+          <<ASSIGN2: forall assign, J assign -> J (LocFun.add loc valw assign)>>;
       FENCE:
         forall tid lang st1 st2
           ordr ordw
@@ -120,11 +120,11 @@ Section Invariant.
       (FIND: IdentMap.find tid ths = Some (existT _ lang st, lc)),
       S tid lang st.
 
-  Definition memory_assign (m:Memory.t) (assign:FLoc.t -> Const.t) :=
+  Definition memory_assign (m:Memory.t) (assign:Loc.t -> Const.t) :=
     forall loc,
     exists from to released,
       Memory.get loc to m =
-      Some (from, Message.full (FLocFun.find loc assign) released).
+      Some (from, Message.full (LocFun.find loc assign) released).
 
   Definition sem_memory (m:Memory.t): Prop :=
     memory_assign m <1= J.
@@ -141,18 +141,18 @@ Section Invariant.
         (STEP: Local.read_step lc1 mem1 loc to val released ord lc2)
         (SEM: sem_memory mem1):
     exists assign,
-      J assign /\ FLocFun.find loc assign = val.
+      J assign /\ LocFun.find loc assign = val.
   Proof.
-    exists (FLocFun.add loc val (FLocFun.init 0)).
+    exists (LocFun.add loc val (LocFun.init 0)).
     splits.
     - apply SEM. ii.
-      destruct (FLoc.eq_dec loc loc0).
-      + subst. rewrite FLocFun.add_spec_eq.
+      destruct (Loc.eq_dec loc loc0).
+      + subst. rewrite LocFun.add_spec_eq.
         inv STEP. esplits; eauto.
-      + rewrite FLocFun.add_spec_neq, FLocFun.init_spec.
+      + rewrite LocFun.add_spec_neq, LocFun.init_spec.
         specialize (INHABITED loc0).
         esplits; eauto. congr.
-    - apply FLocFun.add_spec_eq.
+    - apply LocFun.add_spec_eq.
   Qed.
 
   Lemma sem_memory_write_step_eq
@@ -161,15 +161,15 @@ Section Invariant.
         (INHABITED: Memory.inhabited mem1)
         (STEP: Local.write_step lc1 sc1 mem1 loc from to val releasedm released ord lc2 sc2 mem2 kind)
         (SEM: memory_assign mem2 assign)
-        (LOC: FLocFun.find loc assign = val):
+        (LOC: LocFun.find loc assign = val):
     exists assign0,
       memory_assign mem1 assign0 /\
-      assign = FLocFun.add loc val assign0.
+      assign = LocFun.add loc val assign0.
   Proof.
-    exists (FLocFun.add loc 0 assign). splits; cycle 1.
-    - rewrite FLocFun.add_add_eq. apply FLocFun.ext. i.
-      rewrite FLocFun.add_spec. condtac; subst; ss.
-    - ii. rewrite FLocFun.add_spec. condtac.
+    exists (LocFun.add loc 0 assign). splits; cycle 1.
+    - rewrite LocFun.add_add_eq. apply LocFun.ext. i.
+      rewrite LocFun.add_spec. condtac; subst; ss.
+    - ii. rewrite LocFun.add_spec. condtac.
       { specialize (INHABITED loc0). esplits; eauto. }
       specialize (SEM loc0). des. revert SEM.
       inv STEP. inv WRITE. inv PROMISE; ss.
@@ -191,7 +191,7 @@ Section Invariant.
         assign
         (STEP: Local.write_step lc1 sc1 mem1 loc from to val releasedm released ord lc2 sc2 mem2 kind)
         (SEM: memory_assign mem2 assign)
-        (LOC: FLocFun.find loc assign <> val):
+        (LOC: LocFun.find loc assign <> val):
     memory_assign mem1 assign.
   Proof.
     ii. specialize (SEM loc0). des. revert SEM.
@@ -239,7 +239,7 @@ Section Invariant.
       exploit READ; eauto.
     - exploit WRITE; eauto. i. des.
       esplits; eauto. ii.
-      destruct (Const.eq_dec (FLocFun.find loc x0) val).
+      destruct (Const.eq_dec (LocFun.find loc x0) val).
       { subst. hexploit sem_memory_write_step_eq; eauto. i. des.
         rewrite H0. eauto.
       }
@@ -247,7 +247,7 @@ Section Invariant.
     - exploit sem_memory_read_step; eauto. i. des.
       exploit UPDATE; eauto. i. des.
       esplits; eauto. ii.
-      destruct (Const.eq_dec (FLocFun.find loc x2) valw).
+      destruct (Const.eq_dec (LocFun.find loc x2) valw).
       { subst. hexploit sem_memory_write_step_eq; eauto. i. des.
         rewrite H0. eauto.
       }
@@ -495,8 +495,8 @@ Section Invariant.
                   (@sigT _ (@Language.syntax ProgramEvent.t)) tid program) eqn:X; inv FIND.
       apply inj_pair2 in H1. subst. destruct s. ss.
       eapply ST_INIT; eauto.
-    - ii. cut (x0 = FLocFun.init 0); [by i; subst|].
-      apply FLocFun.ext. i. rewrite FLocFun.init_spec.
+    - ii. cut (x0 = LocFun.init 0); [by i; subst|].
+      apply LocFun.ext. i. rewrite LocFun.init_spec.
       specialize (PR i). des. ss.
       unfold Memory.get, Memory.init in PR. unfold Cell.get, Cell.init in PR. ss.
       apply DOMap.singleton_find_inv in PR. des. inv PR0. auto.
