src/lang/Configuration.v
@@ -80,7 +80,7 @@ Module Threads.
     inv THREAD. ii. esplits; eauto.
   Qed.
 
-  Inductive is_promised tid (loc:FLoc.t) (to:Time.t) (threads:t): Prop :=
+  Inductive is_promised tid (loc:Loc.t) (to:Time.t) (threads:t): Prop :=
   | is_promised_intro
       lang st lc from msg
       (TID: IdentMap.find tid threads = Some (existT _ lang st, lc))
