src/lang/Progress.v
@@ -105,7 +105,7 @@ Proof.
     econs. unfold TView.write_released.
     viewtac; repeat (condtac; viewtac);
       (try by apply Time.bot_spec);
-      (try by unfold TimeMap.singleton, FLocFun.add; condtac; [refl|congr]);
+      (try by unfold TimeMap.singleton, LocFun.add; condtac; [refl|congr]);
       (try by left; eapply TimeFacts.le_lt_lt; [|eauto];
        eapply closed_timemap_max_ts; apply WF1).
     left. eapply TimeFacts.le_lt_lt; [|eauto].
