src/prop/MemoryReorder.v
@@ -173,10 +173,10 @@ Module MemoryReorder.
     erewrite Memory.add_o; eauto. condtac; ss.
     - des. subst. i. des. inv GET. left. splits; eauto.
       inv ADD1. inv ADD. inv LOWER2. inv LOWER.
-      rewrite FLocFun.add_add_eq. econs; auto.
+      rewrite LocFun.add_add_eq. econs; auto.
       unfold Cell.add in *.
       destruct r, r0. ss. subst.
-      unfold FLocFun.add. condtac; [|congr]. s.
+      unfold LocFun.add. condtac; [|congr]. s.
       rewrite DOMap.add_add_eq. econs; auto.
     - guardH o. i. des. right. splits.
       { ii. inv H. unguardH o. des; congr. }
@@ -377,10 +377,10 @@ Module MemoryReorder.
     revert GET. erewrite Memory.split_o; eauto. repeat condtac; ss.
     - des. subst. i. inv GET. left. splits; auto.
       inv SPLIT1. inv SPLIT. inv LOWER2. inv LOWER.
-      rewrite FLocFun.add_add_eq. econs; auto.
+      rewrite LocFun.add_add_eq. econs; auto.
       unfold Cell.split in *.
       destruct r, r0. ss. subst.
-      unfold FLocFun.add. condtac; [|congr]. s.
+      unfold LocFun.add. condtac; [|congr]. s.
       rewrite DOMap.add_add_eq. econs; auto.
     - guardH o. des. subst. congr.
     - guardH o. guardH o0. i. right.
@@ -600,10 +600,10 @@ Module MemoryReorder.
     revert GET. erewrite Memory.lower_o; eauto. condtac; ss.
     - des. subst. i. inv GET. left. splits; eauto.
       inv LOWER1. inv LOWER. inv LOWER2. inv LOWER.
-      rewrite FLocFun.add_add_eq. econs; auto.
+      rewrite LocFun.add_add_eq. econs; auto.
       unfold Cell.lower in *.
       destruct r, r0. ss. subst.
-      unfold FLocFun.add. condtac; [|congr]. s.
+      unfold LocFun.add. condtac; [|congr]. s.
       rewrite DOMap.add_add_eq. econs; auto.
       etrans; eauto.
     - guardH o. i. right. splits.
